spec/prop/vfmDecreasesGasScript.sml
@@ -872,6 +872,7 @@ Proof
   \\ irule decreases_gas_bind_false \\ rw []
   \\ irule decreases_gas_ignore_bind_false
   \\ irule_at Any decreases_gas_consume_gas
+  \\ qexists_tac`F` \\ rw[]
   \\ irule_at Any decreases_gas_ignore_bind_false
   \\ irule_at Any decreases_gas_set_return_data
   \\ irule_at Any decreases_gas_finish
